Source/Core/Parser.cs
@@ -331,7 +331,7 @@ private class BvBounds : Expr {
 				} else SynErr(121);
 				break;
 			}
-			case 51: {
+			case 50: {
 				Implementation(out nnim);
 				Pgm.AddTopLevelDeclaration(nnim); 
 				break;
@@ -677,6 +677,8 @@ private class BvBounds : Expr {
 		ActionDeclRef refinedAction = null;
 		ActionDeclRef invariantAction = null;
 		List<ElimDecl> elims = new List<ElimDecl>();
+		List<Requires> requires = new List<Requires>();
+		List<CallCmd> yieldRequires = new List<CallCmd>();
 		List<Variable> locals;
 		StmtList stmtList;
 		QKeyValue kv = null;
@@ -703,11 +705,11 @@ private class BvBounds : Expr {
 		if (la.kind == 10) {
 			Get();
 			while (StartOf(10)) {
-				SpecAction(ref refinedAction, ref invariantAction, mods, creates, elims);
+				SpecAction(ref refinedAction, ref invariantAction, mods, creates, elims, requires, yieldRequires);
 			}
 		} else if (StartOf(11)) {
 			while (StartOf(10)) {
-				SpecAction(ref refinedAction, ref invariantAction, mods, creates, elims);
+				SpecAction(ref refinedAction, ref invariantAction, mods, creates, elims, requires, yieldRequires);
 			}
 			ImplBody(out locals, out stmtList);
 			impl = new Implementation(name, name.val, new List<TypeVariable>(), Formal.StripWhereClauses(ins), Formal.StripWhereClauses(outs),
@@ -740,7 +742,7 @@ private class BvBounds : Expr {
 		   datatypeTypeCtorDecl.AddConstructor(name, name.val, fields);
 		 }
 		}
-		actionDecl = new ActionDecl(name, name.val, moverType, ins, outs, isPure, creates, refinedAction, invariantAction, elims, mods, datatypeTypeCtorDecl, kv);
+		actionDecl = new ActionDecl(name, name.val, moverType, ins, outs, isPure, creates, refinedAction, invariantAction, elims, requires, yieldRequires, mods, datatypeTypeCtorDecl, kv);
 		
 	}
 
@@ -752,7 +754,7 @@ private class BvBounds : Expr {
 		StmtList/*!*/ stmtList;
 		QKeyValue kv;
 		
-		Expect(51);
+		Expect(50);
 		ProcSignature(false, out x, out typeParams, out ins, out outs, out kv);
 		ImplBody(out locals, out stmtList);
 		impl = new Implementation(x, x.val, typeParams, ins, outs, locals, stmtList, kv, this.errors); 
@@ -1118,15 +1120,24 @@ private class BvBounds : Expr {
 		} else SynErr(132);
 	}
 
-	void SpecAction(ref ActionDeclRef refinedAction, ref ActionDeclRef invariantAction, List<IdentifierExpr> mods, List<ActionDeclRef> creates, List<ElimDecl> elims) {
+	void SpecAction(ref ActionDeclRef refinedAction, ref ActionDeclRef invariantAction, List<IdentifierExpr> mods, List<ActionDeclRef> creates, List<ElimDecl> elims, List<Requires> requires, List<CallCmd> yieldRequires) {
 		if (la.kind == 41) {
-			SpecRefinedAction(ref refinedAction, ref invariantAction);
-		} else if (la.kind == 50) {
+			SpecRefinedAction(ref refinedAction);
+			IToken m; 
+			if (la.kind == 39) {
+				Get();
+				Ident(out m);
+				invariantAction = new ActionDeclRef(m, m.val); 
+			}
+			Expect(10);
+		} else if (la.kind == 52) {
 			SpecModifies(mods);
 		} else if (la.kind == 38) {
 			SpecCreates(creates);
 		} else if (la.kind == 40) {
 			SpecEliminates(elims);
+		} else if (la.kind == 47) {
+			SpecYieldRequires(requires, yieldRequires);
 		} else SynErr(133);
 	}
 
@@ -1168,7 +1179,7 @@ private class BvBounds : Expr {
 		Expect(10);
 	}
 
-	void SpecRefinedAction(ref ActionDeclRef refinedAction, ref ActionDeclRef invariantAction) {
+	void SpecRefinedAction(ref ActionDeclRef refinedAction) {
 		Expect(41);
 		IToken m; 
 		Ident(out m);
@@ -1178,17 +1189,11 @@ private class BvBounds : Expr {
 		 this.SemErr("a refines specification already exists");
 		}
 		
-		if (la.kind == 39) {
-			Get();
-			Ident(out m);
-			invariantAction = new ActionDeclRef(m, m.val); 
-		}
-		Expect(10);
 	}
 
 	void SpecModifies(List<IdentifierExpr> mods) {
 		List<IToken> ms; 
-		Expect(50);
+		Expect(52);
 		if (StartOf(14)) {
 			Idents(out ms);
 			foreach(IToken m in ms) { mods.Add(new IdentifierExpr(m, m.val)); } 
@@ -1196,58 +1201,36 @@ private class BvBounds : Expr {
 		Expect(10);
 	}
 
-	void SpecYieldPrePost(ref ActionDeclRef refinedAction, List<Requires> pre, List<Ensures> post, List<CallCmd> yieldRequires, List<CallCmd> yieldEnsures, List<CallCmd> yieldPreserves, List<IdentifierExpr> mods) {
-		Expr e; Cmd cmd; Token tok = null; QKeyValue kv = null; 
-		if (la.kind == 41) {
-			Get();
-			IToken m; 
-			Ident(out m);
-			if (refinedAction == null) {
-			 refinedAction = new ActionDeclRef(m, m.val);
-			} else {
-			 this.SemErr("a refines specification already exists");
+	void SpecYieldRequires(List<Requires> pre, List<CallCmd> yieldRequires ) {
+		Expr e; Cmd cmd; Token tok; QKeyValue kv = null; 
+		Expect(47);
+		tok = t; 
+		if (StartOf(16)) {
+			while (la.kind == 26) {
+				Attribute(ref kv);
 			}
-			
-		} else if (la.kind == 47) {
-			Get();
-			tok = t; 
-			if (StartOf(16)) {
-				while (la.kind == 26) {
-					Attribute(ref kv);
-				}
-				Proposition(out e);
-				pre.Add(new Requires(tok, false, e, null, kv)); 
-			} else if (la.kind == 36 || la.kind == 52 || la.kind == 65) {
-				CallCmd(out cmd);
-				yieldRequires.Add((CallCmd)cmd); 
-			} else SynErr(134);
-		} else if (la.kind == 48) {
-			Get();
-			tok = t; 
-			if (StartOf(16)) {
-				while (la.kind == 26) {
-					Attribute(ref kv);
-				}
-				Proposition(out e);
-				post.Add(new Ensures(tok, false, e, null, kv)); 
-			} else if (la.kind == 36 || la.kind == 52 || la.kind == 65) {
-				CallCmd(out cmd);
-				yieldEnsures.Add((CallCmd)cmd); 
-			} else SynErr(135);
-		} else if (la.kind == 49) {
-			Get();
-			tok = t; 
+			Proposition(out e);
+			pre.Add(new Requires(tok, false, e, null, kv)); 
+		} else if (la.kind == 36 || la.kind == 51 || la.kind == 65) {
 			CallCmd(out cmd);
-			yieldPreserves.Add((CallCmd)cmd); 
-		} else if (la.kind == 50) {
-			Get();
-			List<IToken> ms; 
-			if (StartOf(14)) {
-				Idents(out ms);
-				foreach(IToken m in ms) { mods.Add(new IdentifierExpr(m, m.val)); } 
-			}
-		} else SynErr(136);
+			yieldRequires.Add((CallCmd)cmd); 
+		} else SynErr(134);
 		Expect(10);
+	}
+
+	void SpecYieldPrePost(ref ActionDeclRef refinedAction, List<Requires> pre, List<Ensures> post, List<CallCmd> yieldRequires, List<CallCmd> yieldEnsures, List<CallCmd> yieldPreserves, List<IdentifierExpr> mods) {
+		if (la.kind == 41) {
+			SpecRefinedAction(ref refinedAction);
+			Expect(10);
+		} else if (la.kind == 47) {
+			SpecYieldRequires(pre, yieldRequires);
+		} else if (la.kind == 48) {
+			SpecYieldEnsures(post, yieldEnsures);
+		} else if (la.kind == 49) {
+			SpecYieldPreserves(yieldPreserves);
+		} else if (la.kind == 52) {
+			SpecModifies(mods);
+		} else SynErr(135);
 	}
 
 	void CallCmd(out Cmd c) {
@@ -1261,7 +1244,7 @@ private class BvBounds : Expr {
 			Get();
 			isAsync = true; 
 		}
-		if (la.kind == 52) {
+		if (la.kind == 51) {
 			Get();
 			isFree = true; 
 		}
@@ -1269,6 +1252,32 @@ private class BvBounds : Expr {
 		x = t; 
 		CallParams(isAsync, isFree, x, out c);
 		
+	}
+
+	void SpecYieldEnsures(List<Ensures> post, List<CallCmd> yieldEnsures ) {
+		Expr e; Cmd cmd; Token tok; QKeyValue kv = null; 
+		Expect(48);
+		tok = t; 
+		if (StartOf(16)) {
+			while (la.kind == 26) {
+				Attribute(ref kv);
+			}
+			Proposition(out e);
+			post.Add(new Ensures(tok, false, e, null, kv)); 
+		} else if (la.kind == 36 || la.kind == 51 || la.kind == 65) {
+			CallCmd(out cmd);
+			yieldEnsures.Add((CallCmd)cmd); 
+		} else SynErr(136);
+		Expect(10);
+	}
+
+	void SpecYieldPreserves(List<CallCmd> yieldPreserves ) {
+		Cmd cmd; Token tok; 
+		Expect(49);
+		tok = t; 
+		CallCmd(out cmd);
+		yieldPreserves.Add((CallCmd)cmd); 
+		Expect(10);
 	}
 
 	void ProcSignature(bool allowWhereClausesOnFormals, out IToken/*!*/ name, out List<TypeVariable>/*!*/ typeParams,
@@ -1291,9 +1300,9 @@ out List<Variable>/*!*/ ins, out List<Variable>/*!*/ outs, out QKeyValue kv) {
 	}
 
 	void Spec(List<Requires> pre, List<IdentifierExpr> mods, List<Ensures> post) {
-		if (la.kind == 50) {
+		if (la.kind == 52) {
 			SpecModifies(mods);
-		} else if (la.kind == 52) {
+		} else if (la.kind == 51) {
 			Get();
 			SpecPrePost(true, pre, post);
 		} else if (la.kind == 47 || la.kind == 48) {
@@ -1441,7 +1450,7 @@ out List<Variable>/*!*/ ins, out List<Variable>/*!*/ outs, out QKeyValue kv) {
 			
 			break;
 		}
-		case 36: case 52: case 65: {
+		case 36: case 51: case 65: {
 			CallCmd(out cn);
 			Expect(10);
 			c = cn; 
@@ -1531,9 +1540,9 @@ out List<Variable>/*!*/ ins, out List<Variable>/*!*/ outs, out QKeyValue kv) {
 		x = t; 
 		Guard(out guard);
 		Contract.Assume(guard == null || cce.Owner.None(guard)); 
-		while (la.kind == 34 || la.kind == 52) {
+		while (la.kind == 34 || la.kind == 51) {
 			isFree = false; z = la/*lookahead token*/; 
-			if (la.kind == 52) {
+			if (la.kind == 51) {
 				Get();
 				isFree = true;  
 			}
@@ -1550,7 +1559,7 @@ out List<Variable>/*!*/ ins, out List<Variable>/*!*/ outs, out QKeyValue kv) {
 				}
 				kv = null;
 				
-			} else if (la.kind == 36 || la.kind == 52 || la.kind == 65) {
+			} else if (la.kind == 36 || la.kind == 51 || la.kind == 65) {
 				CallCmd(out cmd);
 				yields.Add((CallCmd)cmd); 
 			} else SynErr(143);
@@ -2635,24 +2644,24 @@ out QKeyValue kv, out Trigger trig, out Expr/*!*/ body) {
 
 	static readonly bool[,]/*!*/ set = {
 		{_T,_x,_x,_x, _x,_x,_x,_x, _x,_x,_x,_x, _x,_x,_x,_x, _x,_x,_x,_x, _x,_x,_x,_x, _x,_x,_x,_x, _x,_x,_x,_x, _x,_x,_x,_x, _x,_x,_x,_x, _x,_x,_x,_x, _x,_x,_x,_x, _x,_x,_x,_x, _x,_x,_x,_x, _x,_x,_x,_x, _x,_x,_x,_x, _x,_x,_x,_x, _x,_x,_x,_x, _x,_x,_x,_x, _x,_x,_x,_x, _x,_x,_x,_x, _x,_x,_x,_x, _x,_x,_x,_x, _x,_x,_x,_x, _x,_x,_x,_x, _x,_x,_x,_x, _x,_x,_x,_x, _x,_x,_x,_x, _x,_x,_x,_x, _x,_x,_x,_x, _x},
-		{_x,_x,_x,_x, _x,_x,_x,_x, _T,_T,_x,_x, _x,_x,_x,_x, _x,_x,_x,_x, _x,_x,_x,_T, _x,_x,_x,_x, _T,_x,_T,_T, _x,_T,_x,_T, _T,_T,_x,_x, _x,_x,_T,_T, _T,_T,_T,_x, _x,_x,_x,_T, _x,_x,_x,_x, _x,_x,_x,_x, _x,_x,_x,_x, _x,_x,_x,_x, _x,_x,_x,_x, _x,_x,_x,_x, _x,_x,_x,_x, _x,_x,_x,_x, _x,_x,_x,_x, _x,_x,_x,_x, _x,_x,_x,_x, _x,_x,_x,_x, _x,_x,_x,_x, _x,_x,_x,_x, _x,_x,_x,_x, _x,_x,_x,_x, _x,_x,_x,_x, _x},
+		{_x,_x,_x,_x, _x,_x,_x,_x, _T,_T,_x,_x, _x,_x,_x,_x, _x,_x,_x,_x, _x,_x,_x,_T, _x,_x,_x,_x, _T,_x,_T,_T, _x,_T,_x,_T, _T,_T,_x,_x, _x,_x,_T,_T, _T,_T,_T,_x, _x,_x,_T,_x, _x,_x,_x,_x, _x,_x,_x,_x, _x,_x,_x,_x, _x,_x,_x,_x, _x,_x,_x,_x, _x,_x,_x,_x, _x,_x,_x,_x, _x,_x,_x,_x, _x,_x,_x,_x, _x,_x,_x,_x, _x,_x,_x,_x, _x,_x,_x,_x, _x,_x,_x,_x, _x,_x,_x,_x, _x,_x,_x,_x, _x,_x,_x,_x, _x,_x,_x,_x, _x},
 		{_x,_x,_x,_x, _x,_x,_x,_x, _x,_x,_x,_x, _x,_x,_x,_x, _x,_x,_x,_x, _x,_x,_x,_x, _x,_x,_x,_x, _x,_x,_x,_x, _x,_x,_x,_x, _x,_x,_x,_x, _x,_x,_T,_T, _T,_T,_T,_x, _x,_x,_x,_x, _x,_x,_x,_x, _x,_x,_x,_x, _x,_x,_x,_x, _x,_x,_x,_x, _x,_x,_x,_x, _x,_x,_x,_x, _x,_x,_x,_x, _x,_x,_x,_x, _x,_x,_x,_x, _x,_x,_x,_x, _x,_x,_x,_x, _x,_x,_x,_x, _x,_x,_x,_x, _x,_x,_x,_x, _x,_x,_x,_x, _x,_x,_x,_x, _x,_x,_x,_x, _x},
 		{_x,_x,_x,_x, _x,_x,_x,_x, _x,_x,_x,_x, _x,_x,_x,_x, _x,_x,_x,_x, _x,_x,_x,_x, _x,_x,_x,_x, _x,_x,_x,_x, _x,_x,_x,_x, _T,_T,_x,_x, _x,_x,_T,_T, _T,_T,_x,_x, _x,_x,_x,_x, _x,_x,_x,_x, _x,_x,_x,_x, _x,_x,_x,_x, _x,_x,_x,_x, _x,_x,_x,_x, _x,_x,_x,_x, _x,_x,_x,_x, _x,_x,_x,_x, _x,_x,_x,_x, _x,_x,_x,_x, _x,_x,_x,_x, _x,_x,_x,_x, _x,_x,_x,_x, _x,_x,_x,_x, _x,_x,_x,_x, _x,_x,_x,_x, _x,_x,_x,_x, _x},
 		{_x,_T,_x,_x, _x,_x,_x,_x, _x,_x,_x,_T, _x,_x,_x,_x, _T,_T,_T,_T, _x,_T,_x,_x, _x,_x,_T,_x, _x,_x,_x,_x, _x,_x,_x,_x, _x,_x,_x,_x, _x,_x,_T,_T, _T,_T,_x,_x, _x,_x,_x,_x, _x,_x,_x,_x, _x,_x,_x,_x, _x,_x,_x,_x, _x,_x,_x,_x, _x,_x,_x,_x, _x,_x,_x,_x, _x,_x,_x,_x, _x,_x,_x,_x, _x,_x,_x,_x, _x,_x,_x,_x, _x,_x,_x,_x, _x,_x,_x,_x, _x,_x,_x,_x, _x,_x,_x,_x, _x,_x,_x,_x, _x,_x,_x,_x, _x,_x,_x,_x, _x},
 		{_x,_x,_x,_x, _x,_x,_x,_x, _x,_x,_x,_x, _x,_x,_x,_x, _x,_x,_x,_x, _x,_x,_x,_x, _x,_x,_x,_x, _x,_x,_x,_x, _x,_x,_x,_x, _x,_x,_x,_x, _x,_x,_T,_T, _T,_T,_x,_x, _x,_x,_x,_x, _x,_x,_x,_x, _x,_x,_x,_x, _x,_x,_x,_x, _x,_x,_x,_x, _x,_x,_x,_x, _x,_x,_x,_x, _x,_x,_x,_x, _x,_x,_x,_x, _x,_x,_x,_x, _x,_x,_x,_x, _x,_x,_x,_x, _x,_x,_x,_x, _x,_x,_x,_x, _x,_x,_x,_x, _x,_x,_x,_x, _x,_x,_x,_x, _x,_x,_x,_x, _x},
-		{_x,_x,_x,_x, _x,_x,_x,_x, _x,_x,_x,_x, _x,_x,_x,_x, _x,_x,_x,_x, _x,_x,_x,_x, _x,_x,_x,_x, _x,_x,_x,_x, _x,_x,_x,_x, _x,_x,_x,_x, _x,_T,_x,_x, _x,_x,_x,_T, _T,_T,_T,_x, _x,_x,_x,_x, _x,_x,_x,_x, _x,_x,_x,_x, _x,_x,_x,_x, _x,_x,_x,_x, _x,_x,_x,_x, _x,_x,_x,_x, _x,_x,_x,_x, _x,_x,_x,_x, _x,_x,_x,_x, _x,_x,_x,_x, _x,_x,_x,_x, _x,_x,_x,_x, _x,_x,_x,_x, _x,_x,_x,_x, _x,_x,_x,_x, _x,_x,_x,_x, _x},
-		{_x,_x,_x,_x, _x,_x,_x,_x, _x,_x,_x,_x, _x,_x,_x,_x, _x,_x,_x,_x, _x,_x,_x,_x, _x,_x,_T,_x, _x,_x,_x,_x, _x,_x,_x,_x, _x,_x,_x,_x, _x,_T,_x,_x, _x,_x,_x,_T, _T,_T,_T,_x, _x,_x,_x,_x, _x,_x,_x,_x, _x,_x,_x,_x, _x,_x,_x,_x, _x,_x,_x,_x, _x,_x,_x,_x, _x,_x,_x,_x, _x,_x,_x,_x, _x,_x,_x,_x, _x,_x,_x,_x, _x,_x,_x,_x, _x,_x,_x,_x, _x,_x,_x,_x, _x,_x,_x,_x, _x,_x,_x,_x, _x,_x,_x,_x, _x,_x,_x,_x, _x},
-		{_x,_x,_x,_x, _x,_x,_x,_x, _x,_x,_x,_x, _x,_x,_x,_x, _x,_x,_x,_x, _x,_x,_x,_x, _x,_x,_x,_x, _x,_x,_x,_x, _x,_x,_x,_x, _x,_x,_x,_x, _x,_x,_x,_x, _x,_x,_x,_T, _T,_x,_T,_x, _T,_x,_x,_x, _x,_x,_x,_x, _x,_x,_x,_x, _x,_x,_x,_x, _x,_x,_x,_x, _x,_x,_x,_x, _x,_x,_x,_x, _x,_x,_x,_x, _x,_x,_x,_x, _x,_x,_x,_x, _x,_x,_x,_x, _x,_x,_x,_x, _x,_x,_x,_x, _x,_x,_x,_x, _x,_x,_x,_x, _x,_x,_x,_x, _x,_x,_x,_x, _x},
-		{_x,_x,_x,_x, _x,_x,_x,_x, _x,_x,_x,_x, _x,_x,_x,_x, _x,_x,_x,_x, _x,_x,_x,_x, _x,_x,_T,_x, _x,_x,_x,_x, _x,_x,_x,_x, _x,_x,_x,_x, _x,_x,_x,_x, _x,_x,_x,_T, _T,_x,_T,_x, _T,_x,_x,_x, _x,_x,_x,_x, _x,_x,_x,_x, _x,_x,_x,_x, _x,_x,_x,_x, _x,_x,_x,_x, _x,_x,_x,_x, _x,_x,_x,_x, _x,_x,_x,_x, _x,_x,_x,_x, _x,_x,_x,_x, _x,_x,_x,_x, _x,_x,_x,_x, _x,_x,_x,_x, _x,_x,_x,_x, _x,_x,_x,_x, _x,_x,_x,_x, _x},
-		{_x,_x,_x,_x, _x,_x,_x,_x, _x,_x,_x,_x, _x,_x,_x,_x, _x,_x,_x,_x, _x,_x,_x,_x, _x,_x,_x,_x, _x,_x,_x,_x, _x,_x,_x,_x, _x,_x,_T,_x, _T,_T,_x,_x, _x,_x,_x,_x, _x,_x,_T,_x, _x,_x,_x,_x, _x,_x,_x,_x, _x,_x,_x,_x, _x,_x,_x,_x, _x,_x,_x,_x, _x,_x,_x,_x, _x,_x,_x,_x, _x,_x,_x,_x, _x,_x,_x,_x, _x,_x,_x,_x, _x,_x,_x,_x, _x,_x,_x,_x, _x,_x,_x,_x, _x,_x,_x,_x, _x,_x,_x,_x, _x,_x,_x,_x, _x,_x,_x,_x, _x},
-		{_x,_x,_x,_x, _x,_x,_x,_x, _x,_x,_x,_x, _x,_x,_x,_x, _x,_x,_x,_x, _x,_x,_x,_x, _x,_x,_T,_x, _x,_x,_x,_x, _x,_x,_x,_x, _x,_x,_T,_x, _T,_T,_x,_x, _x,_x,_x,_x, _x,_x,_T,_x, _x,_x,_x,_x, _x,_x,_x,_x, _x,_x,_x,_x, _x,_x,_x,_x, _x,_x,_x,_x, _x,_x,_x,_x, _x,_x,_x,_x, _x,_x,_x,_x, _x,_x,_x,_x, _x,_x,_x,_x, _x,_x,_x,_x, _x,_x,_x,_x, _x,_x,_x,_x, _x,_x,_x,_x, _x,_x,_x,_x, _x,_x,_x,_x, _x,_x,_x,_x, _x},
+		{_x,_x,_x,_x, _x,_x,_x,_x, _x,_x,_x,_x, _x,_x,_x,_x, _x,_x,_x,_x, _x,_x,_x,_x, _x,_x,_x,_x, _x,_x,_x,_x, _x,_x,_x,_x, _x,_x,_x,_x, _x,_T,_x,_x, _x,_x,_x,_T, _T,_T,_x,_x, _T,_x,_x,_x, _x,_x,_x,_x, _x,_x,_x,_x, _x,_x,_x,_x, _x,_x,_x,_x, _x,_x,_x,_x, _x,_x,_x,_x, _x,_x,_x,_x, _x,_x,_x,_x, _x,_x,_x,_x, _x,_x,_x,_x, _x,_x,_x,_x, _x,_x,_x,_x, _x,_x,_x,_x, _x,_x,_x,_x, _x,_x,_x,_x, _x,_x,_x,_x, _x},
+		{_x,_x,_x,_x, _x,_x,_x,_x, _x,_x,_x,_x, _x,_x,_x,_x, _x,_x,_x,_x, _x,_x,_x,_x, _x,_x,_T,_x, _x,_x,_x,_x, _x,_x,_x,_x, _x,_x,_x,_x, _x,_T,_x,_x, _x,_x,_x,_T, _T,_T,_x,_x, _T,_x,_x,_x, _x,_x,_x,_x, _x,_x,_x,_x, _x,_x,_x,_x, _x,_x,_x,_x, _x,_x,_x,_x, _x,_x,_x,_x, _x,_x,_x,_x, _x,_x,_x,_x, _x,_x,_x,_x, _x,_x,_x,_x, _x,_x,_x,_x, _x,_x,_x,_x, _x,_x,_x,_x, _x,_x,_x,_x, _x,_x,_x,_x, _x,_x,_x,_x, _x},
+		{_x,_x,_x,_x, _x,_x,_x,_x, _x,_x,_x,_x, _x,_x,_x,_x, _x,_x,_x,_x, _x,_x,_x,_x, _x,_x,_x,_x, _x,_x,_x,_x, _x,_x,_x,_x, _x,_x,_x,_x, _x,_x,_x,_x, _x,_x,_x,_T, _T,_x,_x,_T, _T,_x,_x,_x, _x,_x,_x,_x, _x,_x,_x,_x, _x,_x,_x,_x, _x,_x,_x,_x, _x,_x,_x,_x, _x,_x,_x,_x, _x,_x,_x,_x, _x,_x,_x,_x, _x,_x,_x,_x, _x,_x,_x,_x, _x,_x,_x,_x, _x,_x,_x,_x, _x,_x,_x,_x, _x,_x,_x,_x, _x,_x,_x,_x, _x,_x,_x,_x, _x},
+		{_x,_x,_x,_x, _x,_x,_x,_x, _x,_x,_x,_x, _x,_x,_x,_x, _x,_x,_x,_x, _x,_x,_x,_x, _x,_x,_T,_x, _x,_x,_x,_x, _x,_x,_x,_x, _x,_x,_x,_x, _x,_x,_x,_x, _x,_x,_x,_T, _T,_x,_x,_T, _T,_x,_x,_x, _x,_x,_x,_x, _x,_x,_x,_x, _x,_x,_x,_x, _x,_x,_x,_x, _x,_x,_x,_x, _x,_x,_x,_x, _x,_x,_x,_x, _x,_x,_x,_x, _x,_x,_x,_x, _x,_x,_x,_x, _x,_x,_x,_x, _x,_x,_x,_x, _x,_x,_x,_x, _x,_x,_x,_x, _x,_x,_x,_x, _x,_x,_x,_x, _x},
+		{_x,_x,_x,_x, _x,_x,_x,_x, _x,_x,_x,_x, _x,_x,_x,_x, _x,_x,_x,_x, _x,_x,_x,_x, _x,_x,_x,_x, _x,_x,_x,_x, _x,_x,_x,_x, _x,_x,_T,_x, _T,_T,_x,_x, _x,_x,_x,_T, _x,_x,_x,_x, _T,_x,_x,_x, _x,_x,_x,_x, _x,_x,_x,_x, _x,_x,_x,_x, _x,_x,_x,_x, _x,_x,_x,_x, _x,_x,_x,_x, _x,_x,_x,_x, _x,_x,_x,_x, _x,_x,_x,_x, _x,_x,_x,_x, _x,_x,_x,_x, _x,_x,_x,_x, _x,_x,_x,_x, _x,_x,_x,_x, _x,_x,_x,_x, _x,_x,_x,_x, _x},
+		{_x,_x,_x,_x, _x,_x,_x,_x, _x,_x,_x,_x, _x,_x,_x,_x, _x,_x,_x,_x, _x,_x,_x,_x, _x,_x,_T,_x, _x,_x,_x,_x, _x,_x,_x,_x, _x,_x,_T,_x, _T,_T,_x,_x, _x,_x,_x,_T, _x,_x,_x,_x, _T,_x,_x,_x, _x,_x,_x,_x, _x,_x,_x,_x, _x,_x,_x,_x, _x,_x,_x,_x, _x,_x,_x,_x, _x,_x,_x,_x, _x,_x,_x,_x, _x,_x,_x,_x, _x,_x,_x,_x, _x,_x,_x,_x, _x,_x,_x,_x, _x,_x,_x,_x, _x,_x,_x,_x, _x,_x,_x,_x, _x,_x,_x,_x, _x,_x,_x,_x, _x},
 		{_x,_T,_x,_x, _x,_x,_x,_x, _x,_x,_x,_x, _x,_x,_x,_x, _x,_x,_x,_x, _x,_x,_x,_x, _x,_x,_T,_x, _x,_x,_x,_x, _x,_x,_x,_x, _x,_x,_x,_x, _x,_x,_T,_T, _T,_T,_x,_x, _x,_x,_x,_x, _x,_x,_x,_x, _x,_x,_x,_x, _x,_x,_x,_x, _x,_x,_x,_x, _x,_x,_x,_x, _x,_x,_x,_x, _x,_x,_x,_x, _x,_x,_x,_x, _x,_x,_x,_x, _x,_x,_x,_x, _x,_x,_x,_x, _x,_x,_x,_x, _x,_x,_x,_x, _x,_x,_x,_x, _x,_x,_x,_x, _x,_x,_x,_x, _x,_x,_x,_x, _x},
 		{_x,_x,_x,_x, _x,_x,_x,_x, _x,_x,_x,_T, _x,_x,_x,_x, _T,_T,_T,_x, _x,_x,_x,_x, _x,_x,_x,_x, _x,_x,_x,_x, _x,_x,_x,_x, _x,_x,_x,_x, _x,_x,_x,_x, _x,_x,_x,_x, _x,_x,_x,_x, _x,_x,_x,_x, _x,_x,_x,_x, _x,_x,_x,_x, _x,_x,_x,_x, _x,_x,_x,_x, _x,_x,_x,_x, _x,_x,_x,_x, _x,_x,_x,_x, _x,_x,_x,_x, _x,_x,_x,_x, _x,_x,_x,_x, _x,_x,_x,_x, _x,_x,_x,_x, _x,_x,_x,_x, _x,_x,_x,_x, _x,_x,_x,_x, _x,_x,_x,_x, _x},
 		{_x,_T,_x,_x, _x,_x,_x,_x, _x,_x,_x,_x, _x,_x,_x,_x, _x,_x,_x,_x, _x,_x,_x,_x, _x,_x,_x,_x, _x,_x,_x,_x, _x,_x,_x,_x, _x,_x,_x,_x, _x,_x,_T,_T, _T,_T,_x,_x, _x,_x,_x,_x, _x,_x,_x,_x, _x,_x,_x,_x, _x,_x,_x,_x, _x,_x,_x,_x, _x,_x,_x,_x, _x,_x,_x,_x, _x,_x,_x,_x, _x,_x,_x,_x, _x,_x,_x,_x, _x,_x,_x,_x, _x,_x,_x,_x, _x,_x,_x,_x, _x,_x,_x,_x, _x,_x,_x,_x, _x,_x,_x,_x, _x,_x,_x,_x, _x,_x,_x,_x, _x},
 		{_x,_T,_x,_x, _x,_x,_x,_x, _x,_x,_x,_T, _x,_x,_x,_x, _T,_T,_T,_T, _x,_T,_x,_x, _x,_x,_x,_x, _x,_x,_x,_x, _x,_x,_x,_x, _x,_x,_x,_x, _x,_x,_T,_T, _T,_T,_x,_x, _x,_x,_x,_x, _x,_x,_x,_x, _x,_x,_x,_x, _x,_x,_x,_x, _x,_x,_x,_x, _x,_x,_x,_x, _x,_x,_x,_x, _x,_x,_x,_x, _x,_x,_x,_x, _x,_x,_x,_x, _x,_x,_x,_x, _x,_x,_x,_x, _x,_x,_x,_x, _x,_x,_x,_x, _x,_x,_x,_x, _x,_x,_x,_x, _x,_x,_x,_x, _x,_x,_x,_x, _x},
 		{_x,_T,_T,_T, _T,_T,_T,_T, _x,_x,_x,_T, _x,_x,_x,_x, _T,_T,_x,_x, _x,_x,_x,_x, _x,_x,_T,_x, _x,_x,_x,_x, _x,_x,_x,_x, _x,_x,_x,_x, _x,_x,_T,_T, _T,_T,_x,_x, _x,_x,_x,_x, _x,_x,_x,_T, _x,_x,_x,_x, _x,_x,_x,_x, _x,_x,_x,_x, _x,_x,_x,_x, _x,_x,_x,_x, _x,_x,_x,_x, _x,_x,_x,_x, _x,_x,_x,_T, _x,_x,_x,_x, _x,_T,_T,_T, _T,_T,_T,_T, _T,_T,_T,_T, _T,_T,_T,_T, _T,_x,_x,_x, _x,_x,_x,_x, _x,_x,_x,_x, _x},
-		{_x,_T,_x,_x, _x,_x,_x,_x, _x,_x,_x,_x, _x,_x,_x,_x, _x,_x,_x,_x, _x,_x,_x,_x, _x,_x,_x,_x, _x,_x,_x,_x, _x,_x,_x,_x, _T,_x,_x,_x, _x,_x,_T,_T, _T,_T,_x,_x, _x,_x,_x,_x, _T,_T,_T,_T, _x,_T,_x,_T, _T,_T,_T,_x, _x,_T,_T,_x, _x,_x,_x,_x, _x,_x,_x,_x, _x,_x,_x,_x, _x,_x,_x,_x, _x,_x,_x,_x, _x,_x,_x,_x, _x,_x,_x,_x, _x,_x,_x,_x, _x,_x,_x,_x, _x,_x,_x,_x, _x,_x,_x,_x, _x,_x,_x,_x, _x,_x,_x,_x, _x},
-		{_x,_T,_x,_x, _x,_x,_x,_x, _x,_x,_x,_x, _x,_x,_x,_x, _x,_x,_x,_x, _x,_x,_x,_x, _x,_x,_x,_x, _x,_x,_x,_x, _x,_x,_x,_x, _T,_x,_x,_x, _x,_x,_T,_T, _T,_T,_x,_x, _x,_x,_x,_x, _T,_x,_x,_x, _x,_x,_x,_x, _T,_T,_T,_x, _x,_T,_T,_x, _x,_x,_x,_x, _x,_x,_x,_x, _x,_x,_x,_x, _x,_x,_x,_x, _x,_x,_x,_x, _x,_x,_x,_x, _x,_x,_x,_x, _x,_x,_x,_x, _x,_x,_x,_x, _x,_x,_x,_x, _x,_x,_x,_x, _x,_x,_x,_x, _x,_x,_x,_x, _x},
+		{_x,_T,_x,_x, _x,_x,_x,_x, _x,_x,_x,_x, _x,_x,_x,_x, _x,_x,_x,_x, _x,_x,_x,_x, _x,_x,_x,_x, _x,_x,_x,_x, _x,_x,_x,_x, _T,_x,_x,_x, _x,_x,_T,_T, _T,_T,_x,_x, _x,_x,_x,_T, _x,_T,_T,_T, _x,_T,_x,_T, _T,_T,_T,_x, _x,_T,_T,_x, _x,_x,_x,_x, _x,_x,_x,_x, _x,_x,_x,_x, _x,_x,_x,_x, _x,_x,_x,_x, _x,_x,_x,_x, _x,_x,_x,_x, _x,_x,_x,_x, _x,_x,_x,_x, _x,_x,_x,_x, _x,_x,_x,_x, _x,_x,_x,_x, _x,_x,_x,_x, _x},
+		{_x,_T,_x,_x, _x,_x,_x,_x, _x,_x,_x,_x, _x,_x,_x,_x, _x,_x,_x,_x, _x,_x,_x,_x, _x,_x,_x,_x, _x,_x,_x,_x, _x,_x,_x,_x, _T,_x,_x,_x, _x,_x,_T,_T, _T,_T,_x,_x, _x,_x,_x,_T, _x,_x,_x,_x, _x,_x,_x,_x, _T,_T,_T,_x, _x,_T,_T,_x, _x,_x,_x,_x, _x,_x,_x,_x, _x,_x,_x,_x, _x,_x,_x,_x, _x,_x,_x,_x, _x,_x,_x,_x, _x,_x,_x,_x, _x,_x,_x,_x, _x,_x,_x,_x, _x,_x,_x,_x, _x,_x,_x,_x, _x,_x,_x,_x, _x,_x,_x,_x, _x},
 		{_x,_T,_T,_T, _T,_T,_T,_T, _x,_x,_x,_T, _x,_x,_x,_x, _T,_T,_x,_x, _x,_x,_x,_x, _x,_x,_x,_x, _x,_x,_x,_x, _x,_x,_x,_x, _x,_x,_x,_x, _x,_x,_T,_T, _T,_T,_x,_x, _x,_x,_x,_x, _x,_x,_x,_T, _x,_x,_x,_x, _x,_x,_x,_x, _x,_x,_x,_x, _x,_x,_x,_x, _x,_x,_x,_x, _x,_x,_x,_x, _x,_x,_x,_x, _x,_x,_x,_T, _x,_x,_x,_x, _x,_T,_T,_T, _T,_T,_T,_T, _T,_T,_T,_T, _T,_T,_T,_T, _T,_x,_x,_x, _x,_x,_x,_x, _x,_x,_x,_x, _x},
 		{_x,_x,_x,_x, _x,_x,_x,_x, _x,_x,_x,_x, _x,_x,_T,_x, _x,_x,_x,_T, _x,_x,_x,_x, _x,_x,_x,_x, _x,_x,_x,_x, _x,_x,_x,_x, _x,_x,_x,_x, _x,_x,_x,_x, _x,_x,_x,_x, _x,_x,_x,_x, _x,_x,_x,_x, _x,_x,_x,_x, _x,_x,_x,_T, _T,_x,_x,_x, _x,_x,_x,_x, _x,_x,_x,_x, _x,_x,_x,_x, _x,_x,_x,_x, _x,_x,_x,_x, _x,_x,_x,_x, _x,_x,_x,_x, _x,_x,_x,_x, _x,_x,_x,_x, _x,_x,_x,_x, _x,_x,_x,_x, _x,_x,_x,_x, _x,_x,_x,_x, _x},
 		{_x,_x,_x,_x, _x,_x,_x,_x, _x,_x,_x,_x, _x,_x,_x,_x, _x,_x,_x,_x, _x,_x,_x,_x, _x,_x,_x,_x, _x,_x,_x,_x, _x,_x,_x,_x, _x,_x,_x,_x, _x,_x,_x,_x, _x,_x,_x,_x, _x,_x,_x,_x, _x,_x,_x,_x, _x,_x,_x,_x, _x,_x,_x,_x, _x,_x,_x,_x, _x,_x,_T,_T, _T,_T,_x,_x, _x,_x,_x,_x, _x,_x,_x,_x, _x,_x,_x,_x, _x,_x,_x,_x, _x,_x,_x,_x, _x,_x,_x,_x, _x,_x,_x,_x, _x,_x,_x,_x, _x,_x,_x,_x, _x,_x,_x,_x, _x,_x,_x,_x, _x},
@@ -2735,9 +2744,9 @@ public class Errors {
 			case 47: s = "\"requires\" expected"; break;
 			case 48: s = "\"ensures\" expected"; break;
 			case 49: s = "\"preserves\" expected"; break;
-			case 50: s = "\"modifies\" expected"; break;
-			case 51: s = "\"implementation\" expected"; break;
-			case 52: s = "\"free\" expected"; break;
+			case 50: s = "\"implementation\" expected"; break;
+			case 51: s = "\"free\" expected"; break;
+			case 52: s = "\"modifies\" expected"; break;
 			case 53: s = "\"goto\" expected"; break;
 			case 54: s = "\"return\" expected"; break;
 			case 55: s = "\"if\" expected"; break;
@@ -2819,9 +2828,9 @@ public class Errors {
 			case 131: s = "invalid TypeArgs"; break;
 			case 132: s = "invalid MoverQualifier"; break;
 			case 133: s = "invalid SpecAction"; break;
-			case 134: s = "invalid SpecYieldPrePost"; break;
+			case 134: s = "invalid SpecYieldRequires"; break;
 			case 135: s = "invalid SpecYieldPrePost"; break;
-			case 136: s = "invalid SpecYieldPrePost"; break;
+			case 136: s = "invalid SpecYieldEnsures"; break;
 			case 137: s = "invalid Spec"; break;
 			case 138: s = "invalid SpecPrePost"; break;
 			case 139: s = "invalid LabelOrCmd"; break;
